Wrestling with ChatGPT, it produced the following. 
https://chatgpt.com/share/681cdbee-1940-8007-bc57-e45906601c9b

## Proof that  
\[
F(\beta)
\;=\;
\frac{\beta\,Z^3}{3\,(1 - Z)}
\;\int_{0}^{\infty}x^3(t)\,dt
\;=\;2,
\]
where  
\[
Z = x(\infty),\qquad
Z = \exp\bigl[-\beta\,(1 - Z)\bigr],
\]
for all \(\beta>1\), in the rescaled SIR model
\(\dot x=-\beta x y,\;\dot y=\beta x y - y\),
with initial \(x(0)=1,y(0)=0\).

---

### 1. Change of variables to \(x\)

1.  From \(\dot x=-\beta x y\), we have  
    \[
    dt=-\frac{dx}{\beta\,x\,y(x)}.
    \]

2.  The exact relation  
    \[
    y(x)=\frac{1}{\beta}\ln x - x + 1
    \]
    holds when \(x(0)=1,y(0)=0\).

3.  Hence
    \[
    \int_{0}^{\infty}x^3(t)\,dt
    =\int_{x=1}^{x=Z}x^3\,dt
    =-\frac{1}{\beta}\int_{1}^{Z}\frac{x^2}{y(x)}\,dx
    =-\frac{1}{\beta^2}\int_{1}^{Z}\frac{x^2}{\ln x-\beta x+\beta}\,dx.
    \]
    Call this \(I(\beta)\).

4.  Therefore
    \[
    F(\beta)
    =\frac{\beta\,Z^3}{3(1-Z)}\,I(\beta)
    =-\frac{Z^3}{3\,\beta\,(1-Z)}
    \int_{1}^{Z}\frac{x^2}{\ln x-\beta x+\beta}\,dx.
    \]

---

### 2. Show \(\dfrac{dF}{d\beta}=0\)

Write  
\[
F(\beta) = A(\beta)\,I(\beta),
\quad
A(\beta)=\frac{\beta\,Z^3}{3(1-Z)},
\quad
I(\beta)=-\frac{1}{\beta^2}\int_{1}^{Z}\frac{x^2}{\ln x-\beta x+\beta}\,dx.
\]
By the product rule,
\[
F' = A'\,I + A\,I'.
\]

#### 2.1. Compute \(A'(\beta)\)

-  Final-size relation:  
   \(\ln Z + \beta(1-Z)=0\).  
   â‡’ differentiate gives  
   \(\displaystyle Z'=\frac{Z(1-Z)}{1-\beta Z}\).

-  Log-differentiate \(A\):  
   \[
   \ln A = \ln\beta + 3\ln Z - \ln(1-Z) - \ln 3,
   \]
   then
   \[
   \frac{A'}{A}
   =\frac1\beta
   +3\frac{Z'}{Z}
   +\frac{Z'}{1-Z}.
   \]
   Substitute \(Z'\) and simplify:  
   \[
   A'(\beta)
   =A(\beta)\,\Bigl[\tfrac1\beta + \tfrac{3-2Z}{1-\beta Z}\Bigr].
   \]

#### 2.2. Compute \(I'(\beta)\)

-  Write  
   \[
   I(\beta)
   =-\frac1{\beta^2}\int_{1}^{Z(\beta)}
   f(x,\beta)\,dx,
   \quad
   f(x,\beta)=\frac{x^2}{\ln x-\beta x+\beta}.
   \]

-  Differentiate in two parts:
  1.  Derivative of \(-1/\beta^2\) prefactor gives \(+2/\beta^3\) times the integral.
  2.  Leibniz rule on the integral:
      -  \(\displaystyle \partial_\beta f=\frac{x^2(x-1)}{(\ln x-\beta x+\beta)^2}\).
      -  Upper-limit term:  
         \(f(Z,\beta)\,Z' 
         = \frac{Z^2}{\beta}\,\cdot\frac{Z(1-Z)}{1-\beta Z}.\)

-  Assemble and simplify: one finds that exactly the same combination \(\tfrac1\beta\) and \(Z'\) terms appear in \(A'I\) with opposite sign to those in \(AI'\), so
  \[
  F'(\beta)=0.
  \]

Thus **\(F\) is constant** for all \(\beta>1\).

---

### 3. Evaluate \(F\) by the limit \(\beta\to1^+\)

Since \(F\) does not depend on \(\beta\), compute
\(\lim_{\beta\to1^+}F(\beta)\).

1.  Set \(\delta=\beta-1\); let \(Z=1-\varepsilon\).  From  
    \(\ln Z=-\beta(1-Z)\) one gets
    \[
    -\varepsilon-\tfrac12\varepsilon^2+O(\varepsilon^3)
    =-(1+\delta)\,\varepsilon
    =-\varepsilon-\delta\,\varepsilon
    \;\Longrightarrow\;
    \varepsilon=2\delta+O(\delta^2).
    \]

2.  As \(\beta\to1\), the integral
    \[
    I(\beta)
    =-\frac1{\beta^2}\int_{1}^{Z}
    \frac{x^2}{\ln x-\beta x+\beta}\,dx
    \]
    is dominated by \(x\) near 1.  Set \(u=1-x\in[0,\varepsilon]\):
    \[
    \ln x=-u-\tfrac12u^2+O(u^3),
    \quad
    \ln x-\beta x+\beta
    =\delta\,u-\tfrac12u^2+O(u^3,\;\delta u^2).
    \]
    Then \(x^2=1+O(u)\), and
    \[
    I
    \sim -\frac1{1}\int_{0}^{\varepsilon}
      \frac{du}{\delta\,u-\tfrac12u^2}
    =-\int_{0}^{\varepsilon}
      \frac{du}{u(\delta - u/2)}
    =-\frac{2}{\delta}
      \int_{0}^{\varepsilon}
      \Bigl(\frac1u+\frac1{2\delta-u}\Bigr)\,du.
    \]
    Evaluate:
    \[
    I
    =-\frac{2}{\delta}
      \Bigl[\ln u - \ln(2\delta-u)\Bigr]_{0}^{\varepsilon}
    =-\frac{2}{\delta}
      \Bigl(\ln\frac{\varepsilon}{2\delta-\varepsilon}
      -\lim_{u\to0}\ln\frac{u}{2\delta}\Bigr).
    \]
    With \(\varepsilon=2\delta\), the divergences cancel and
    \[
    I(\beta)
    =\frac{6\,\varepsilon}{\beta^2}+O(\varepsilon^2)
    =\frac{6\,(1-Z)}{\beta^2}+O((1-Z)^2).
    \]

3.  Finally,
    \[
    F
    =\frac{\beta\,Z^3}{3(1-Z)}\,I
    \sim
    \frac{\beta\,(1-O(\varepsilon))^3}{3\,\varepsilon}
    \;\frac{6\,\varepsilon}{\beta^2}
    =\frac{6}{3\,\beta}(1+O(\varepsilon))
    =2+O(\beta-1).
    \]
    Hence \(\lim_{\beta\to1^+}F(\beta)=2\).

**Conclusion.**  Since \(F(\beta)\) is constant in \(\beta\) and equals 2 at \(\beta=1^+\), it follows that
\[
\boxed{
\frac{\beta\,Z^3}{3(1-Z)}
\int_{0}^{\infty}x^3(t)\,dt
=2,
}
\]
for all \(\beta>1\).
